@prefix :  <http://www.purl.org/twc/ns/darkdata#> .
@prefix dd:  <http://www.purl.org/twc/ns/darkdata#> .
@prefix owl:  <http://www.w3.org/2002/07/owl#> .
@prefix rdf:  <http://www.w3.org/1999/02/22-rdf-syntax-ns#> .
@prefix xml:  <http://www.w3.org/XML/1998/namespace> .
@prefix xsd:  <http://www.w3.org/2001/XMLSchema#> .
@prefix rdfs:  <http://www.w3.org/2000/01/rdf-schema#> .
@prefix oml:  <http://def.seegrid.csiro.au/ontology/om/om-lite#> .

<http://www.purl.org/twc/ns/darkdata>
        rdf:type     owl:Ontology ;
        rdfs:label   "Dark Data Ontology"@en ;
        owl:imports  <http://def.seegrid.csiro.au/ontology/om/om-lite> .

dd:topic
        rdf:type owl:AnnotationProperty ;
        rdfs:label "topic" ;
        rdfs:comment "keyword associated with this class or property" .

dd:observableProperty
        rdf:type      owl:ObjectProperty ;
        rdfs:label    "observable property"@en ;
        rdfs:comment  "observable property of some physical manifestation of a phenomena"@en ;
        rdfs:range    dd:ObservableProperty ;
        rdfs:domain   dd:PhysicalManifestation .

dd:physicalDriver  rdf:type  owl:ObjectProperty ;
        rdfs:label    "physical driver"@en ;
        rdfs:comment  "physical manifestation that is a driving force for a phenomena (e.g. elevated sea surface temperature is a driver of hurricanes)"@en ;
        rdfs:domain   dd:Phenomena ;
        rdfs:range    dd:PhysicalManifestation .

dd:physicalManifestation
        rdf:type      owl:ObjectProperty ;
        rdfs:label    "physical manifestation"@en ;
        rdfs:comment  "physical manifestation of a phenomena"@en ;
        rdfs:domain   dd:Phenomena ;
        rdfs:range    dd:PhysicalManifestation .

dd:AerosolOpticalDepth
        rdf:type         owl:Class ;
        rdfs:label       "Aerosol Optical Depth"@en ;
        rdfs:subClassOf  dd:ObservableProperty .

dd:AshPlume  rdf:type    owl:Class ;
        rdfs:label       "Ash Plume"@en ;
        rdfs:subClassOf  dd:PhysicalManifestation .

dd:AtmosphericConcentration
        rdf:type         owl:Class ;
        rdfs:label       "Atmospheric Concentration"@en ;
        rdfs:subClassOf  dd:ObservableProperty .

dd:Column_SO2  rdf:type  owl:Class ;
        rdfs:label       "SO2 Column"@en ;
        rdfs:subClassOf  dd:ObservableProperty .

dd:DataVariable  rdf:type  owl:Class ;
        rdfs:label    "Data Variable"@en ;
        rdfs:comment  "Representation of the measurement in a data file"@en .

dd:DataVariableObservation
        rdf:type         owl:Class ;
        rdfs:label       "Data Variable Observation"@en ;
        rdfs:subClassOf  oml:Observation .

_:b0    rdf:type           owl:Restriction ;
        owl:onProperty     oml:result ;
        owl:allValuesFrom  dd:DataVariable .

dd:DataVariableObservation
        rdfs:subClassOf  _:b0 ;
        rdfs:comment     "Observation whose result is a data variable"@en .

dd:ElevatedSurfaceTemperature
        rdf:type         owl:Class ;
        rdfs:label       "Elevated Surface Temperature"@en ;
        rdfs:subClassOf  dd:PhysicalManifestation .

dd:Emission_SO2  rdf:type  owl:Class ;
        rdfs:label       "SO2 Emission"@en ;
        rdfs:subClassOf  dd:PhysicalManifestation .

dd:Event  rdf:type  owl:Class ;
        rdfs:label  "Event"@en .

dd:Histogram  rdf:type   owl:Class ;
        rdfs:label       "Histogram"@en ;
        rdfs:subClassOf  dd:Visualization .

dd:Hovmoller  rdf:type   owl:Class ;
        rdfs:label       "Hovmoller"@en ;
        rdfs:subClassOf  dd:Visualization .

dd:HurricaneEye  rdf:type  owl:Class ;
        rdfs:label       "Hurricane Eye"@en ;
        rdfs:subClassOf  dd:PhysicalManifestation .

dd:ObservableProperty
        rdf:type    owl:Class ;
        rdfs:label  "Observable Property"@en .

dd:Phenomena  rdf:type   owl:Class ;
        rdfs:label       "Phenomena"@en ;
        rdfs:subClassOf  dd:Event ;
        rdfs:comment     "An observable occurrence of particular physical (as opposed to dynamic or synoptic) significance within the atmosphere"@en .

dd:PhysicalManifestation
        rdf:type    owl:Class ;
        rdfs:label  "Physical Manifestation"@en .

_:b3    rdf:type            owl:Restriction ;
        owl:onProperty      dd:observableProperty ;
        owl:someValuesFrom  dd:AerosolOpticalDepth .

dd:PhysicalManifestation
        rdfs:subClassOf  _:b3 .

dd:Radiance  rdf:type    owl:Class ;
        rdfs:label       "Radiance"@en ;
        rdfs:subClassOf  dd:ObservableProperty .

dd:RainRate  rdf:type    owl:Class ;
        rdfs:label       "Rain Rate"@en ;
        rdfs:subClassOf  dd:ObservableProperty .

dd:SeasonalTimeSeries
        rdf:type         owl:Class ;
        rdfs:label       "Seasonal Time-Series"@en ;
        rdfs:subClassOf  dd:Visualization .

dd:Temperature  rdf:type  owl:Class ;
        rdfs:label       "Temperature"@en ;
        rdfs:subClassOf  dd:ObservableProperty .

dd:TimeAveragedMap  rdf:type  owl:Class ;
        rdfs:label       "Time-averaged Map"@en ;
        rdfs:subClassOf  dd:Visualization .

dd:UserDefinedClimatology
        rdf:type         owl:Class ;
        rdfs:label       "User-defined Climatology"@en ;
        rdfs:subClassOf  dd:Visualization .

dd:VerticalProfile  rdf:type  owl:Class ;
        rdfs:label       "Vertical Profile"@en ;
        rdfs:subClassOf  dd:Visualization .

dd:Visualization  rdf:type  owl:Class ;
        rdfs:label  "Visualization"@en .

dd:WindFields  rdf:type  owl:Class ;
        rdfs:label       "Wind Fields"@en ;
        rdfs:subClassOf  dd:PhysicalManifestation .

dd:ZonalMeans  rdf:type  owl:Class ;
        rdfs:label       "Zonal Means"@en ;
        rdfs:subClassOf  dd:Visualization .

dd:aerosol_optical_depth_thickness
        rdf:type  dd:AerosolOpticalDepth ;
        rdf:type  owl:NamedIndividual .

dd:atmospheric_concentration_SO2
        rdf:type  dd:AtmosphericConcentration ;
        rdf:type  owl:NamedIndividual .

dd:infrared_radiance  rdf:type  dd:Radiance ;
        rdf:type  owl:NamedIndividual .

dd:surface_temperature
        rdf:type  dd:Temperature ;
        rdf:type  owl:NamedIndividual .

dd:visible_radiance  rdf:type  dd:Radiance ;
        rdf:type  owl:NamedIndividual .

# Giovanni Visualization instances

dd:DiArAvTs  rdf:type  dd:Visualization ;
        rdfs:comment  "Time series of area averages of differences between two variables at each spatial grid point"@en .

dd:HvLt  rdf:type     dd:Visualization ;
        rdf:type      dd:Hovmoller ;
        rdfs:comment  "Longitude-averaged Hovmoller, plotted over the selected time and longitude ranges"@en .

dd:HiGm  rdf:type     dd:Visualization ;
        rdfs:comment  "Distribution of values over time and space"@en .

dd:TmAvSc  rdf:type   dd:Visualization ;
        rdfs:comment  "Time-averaged, interactive X-Y plot of 2 variables"@en .

dd:ArAvTs  rdf:type   dd:Visualization ;
        rdfs:comment  "Time series of area-averaged values"@en .

dd:CoMp  rdf:type     dd:Visualization ;
        rdfs:comment  "Simple linear regression of 2 variables at each grid cell"@en .

dd:TmAvMp  rdf:type   dd:Visualization ;
        rdfs:comment  "Interactive map of average over time at each grid cell"@en .

dd:MpAn  rdf:type     dd:Visualization ;
        rdfs:comment  "Map animated along the chosen timeline for each grid cell"@en .

dd:StSc  rdf:type     dd:Visualization ;
        rdfs:comment  "Static Scatter plot"@en .

dd:VtPf  rdf:type     dd:Visualization ;
        rdfs:comment  "Vertical Profile"@en .

dd:HvLn  rdf:type     dd:Visualization ;
        rdf:type      dd:Hovmoller ;
        rdfs:comment  "Latitude-averaged Hovmoller, plotted over the selected time and latitude ranges"@en .

dd:QuCl  rdf:type     dd:Visualization ;
        rdfs:comment  "Quasi Climatology Map"@en .

dd:InTs  rdf:type     dd:Visualization ;
        rdfs:comment  "Seasonal (inter annual) time series"@en .

dd:DiTmAvMp  rdf:type  dd:Visualization ;
        rdfs:comment  "Difference of two time averaged variable maps"@en .

dd:IaSc  rdf:type     dd:Visualization ;
        rdfs:comment  "Interactive Scatter Plot"@en .

dd:AcMp  rdf:type     dd:Visualization ;
        rdfs:comment  "Accumulation of measurement over time at each grid point"@en .

dd:ArAvSc  rdf:type   dd:Visualization ;
        rdfs:comment  "Scatter plot comparing area averaged time series for two variables"@en .

dd:CrTm  rdf:type     dd:Visualization ;
        rdfs:comment  "Cross Map, Time-Pressure"@en .

dd:CrLt  rdf:type     dd:Visualization ;
        rdfs:comment  "Cross Map, Latitude-Pressure"@en .

dd:CrLn  rdf:type     dd:Visualization ;
        rdfs:comment  "Cross Map, Longitude-Pressure"@en .

dd:ZnMn  rdf:type     dd:Visualization ;
        rdfs:comment  "Zonal mean plot, averaged values are plotted over latitude zones"@en .

# Phenomena sub-classes
# aligned with eonet event topic categories (some topic categories contain more than one phenomena subclass)

dd:SevereStorm
        rdf:type owl:Class ;
        rdfs:label "Severe Storm"@en ;
        rdfs:subClassOf dd:Phenomena ;
        rdfs:subClassOf [
                rdf:type            owl:Restriction ;
                owl:onProperty      dd:physicalManifestation ;
                owl:someValuesFrom  dd:WindFields ;
        ];
        dd:topic "Severe Storms" ;
        rdfs:seeAlso <http://eonet.sci.gsfc.nasa.gov/api/v1/topics/10> .

dd:Hurricane
        rdf:type owl:Class ;
        rdfs:label "Hurricane"@en ;
        rdfs:subClassOf dd:SevereStorm ;
        rdfs:subClassOf [
                rdf:type            owl:Restriction ;
                owl:onProperty      dd:physicalManifestation ;
                owl:someValuesFrom  dd:HurricaneEye ;
        ] ;
        dd:topic "Hurrcane" ;
        rdfs:seeAlso <http://eonet.sci.gsfc.nasa.gov/api/v1/topics/10> .

dd:Flood
        rdf:type owl:Class ;
        rdfs:label "Flood"@en;
        rdfs:subClassOf dd:Phenomena ;
        dd:topic "Floods" ;
        rdfs:seeAlso <http://eonet.sci.gsfc.nasa.gov/api/v1/topics/9> .

dd:Wildfire
        rdf:type owl:Class ;
        rdfs:label "Wildfire"@en;
        rdfs:subClassOf dd:Phenomena ;
        dd:topic "Wildfires" ;
        rdfs:seeAlso <http://eonet.sci.gsfc.nasa.gov/api/v1/topics/8> .

dd:DustAndHaze
        rdf:type owl:Class ;
        rdfs:label "Wildfire"@en ;
        rdfs:subClassOf dd:Phenomena ;
        dd:topic "Dust and Haze" ;
        rdfs:seeAlso <http://eonet.sci.gsfc.nasa.gov/api/v1/topics/7> .

dd:DustStorm
        rdf:type owl:Class ;
        rdfs:label "Dust Storm" ;
        rdfs:subClassOf dd:DustAndHaze, dd:SevereStorm ;
        dd:topic "Dust Storm" .

dd:Drought
        rdf:type owl:Class ;
        rdfs:label "Drought"@en;
        rdfs:label "Long lasting absence of precipitation affecting agriculture and livestock, and the overall availability of food and water." ;
        rdfs:subClassOf dd:Phenomena ;
        dd:topic "Drought" ;
        rdfs:seeAlso <http://eonet.sci.gsfc.nasa.gov/api/v1/topics/6> .

dd:VolcanicEruption
        rdf:type owl:Class ;
        rdfs:label "Volcanic Eruption"@en;
        rdfs:comment "Related to both the physical effects of an eruption (rock, ash, lava) and the atmospheric (ash and gas plumes). " ;
        rdfs:subClassOf dd:Phenomena ;
        dd:topic "Volcanoes" ;
        rdfs:subClassOf [
                rdf:type owl:Restriction ;
                owl:onProperty dd:physicalManifestation ;
                owl:someValuesFrom dd:AshPlume ;
        ] ;
        rdfs:seeAlso <http://eonet.sci.gsfc.nasa.gov/api/v1/topics/12> .

dd:WaterColor
        rdf:type owl:Class ;
        rdfs:label "Water Color"@en;
        rdfs:comment "Related to events that alter the appearance of water: phytoplankton, red tide, algae, sediment, whiting, etc." ;
        rdfs:subClassOf dd:Phenomena ;
        dd:topic "Water Color" ;
        rdfs:seeAlso <http://eonet.sci.gsfc.nasa.gov/api/v1/topics/13> .

dd:Landslide
        rdf:type owl:Class ;
        rdfs:label "Landslide"@en ;
        rdfs:comment "Related to landslides and variations thereof: mudslides, avalanche." ;
        rdfs:subClassOf dd:Phenomena ;
        dd:topic "Landslides" ;
        rdfs:seeAlso <http://eonet.sci.gsfc.nasa.gov/api/v1/topics/14> .

dd:SeaAndLakeIce
        rdf:type owl:Class ;
        rdfs:label "Sea and Lake Ice"@en ;
        rdfs:comment "Related to all ice that resides on oceans and lakes, including sea and lake ice (permanent and seasonal) and icebergs." ;
        rdfs:subClassOf dd:Phenomena ;
        dd:topic "Sea and Lake Ice" ;
        rdfs:seeAlso <http://eonet.sci.gsfc.nasa.gov/api/v1/topics/15> .

dd:Earthquake
        rdf:type owl:Class ;
        rdfs:label "Earthquake"@en ;
        rdfs:comment "Related to all manner of shaking and displacement. Certain aftermath of earthquakes may also be found under landslides and floods." ;
        rdfs:subClassOf dd:Phenomena ;
        dd:topic "Earthquakes" ;
        rdfs:seeAlso <http://eonet.sci.gsfc.nasa.gov/api/v1/topics/16> .

dd:Snow
        rdf:type owl:Class ;
        rdfs:label "Snow"@en ;
        rdfs:comment "Related to snow events, particularly extreme/anomalous snowfall in either timing or extent/depth." ;
        rdfs:subClassOf dd:Phenomena ;
        dd:topic "Snow" ;
        rdfs:seeAlso <http://eonet.sci.gsfc.nasa.gov/api/v1/topics/17> .

dd:TemperatureExtreme
        rdf:type owl:Class ;
        rdfs:label "Temperature Extreme"@en ;
        rdfs:comment "Related to anomalous land temperatures, either heat or cold." ;
        rdfs:subClassOf dd:Phenomena ;
        dd:topic "Temperature Extremes" ;
        rdfs:seeAlso <http://eonet.sci.gsfc.nasa.gov/api/v1/topics/18> .

dd:ManMade
        rdf:type owl:Class ;
        rdfs:label "Man-made"@en ;
        rdfs:comment "Events that have been human-induced and are extreme in their extent." ;
        rdfs:subClassOf dd:Phenomena ;
        dd:topic "Manmade" ;
        rdfs:seeAlso <http://eonet.sci.gsfc.nasa.gov/api/v1/topics/19> .
